Define free variable notions for f.o. terms and formulas.

examples/logic/foltypesScript.sml
@@ -33,7 +33,9 @@ val lp = ``
 ``
 
 val {term_ABS_pseudo11, term_REP_11, genind_term_REP, genind_exists,
-     termP, absrep_id, repabs_pseudo_id, term_REP_t, term_ABS_t,
+     termP, absrep_id = term_absrep_id,
+     repabs_pseudo_id = term_repabs_pseudo_id,
+     term_REP_t, term_ABS_t,
      newty = term_ty, ...} =
     new_type_step1 tyname 0 {vp=vp, lp = lp}
 
@@ -70,8 +72,8 @@ val tpm_name_pfx = "t"
 val {tpm_thm = tpm_thm0, term_REP_tpm, t_pmact_t, tpm_t} =
     define_permutation { name_pfx = "t", name = tyname,
                          term_REP_t = term_REP_t,
-                         term_ABS_t = term_ABS_t, absrep_id = absrep_id,
-                         repabs_pseudo_id = repabs_pseudo_id,
+                         term_ABS_t = term_ABS_t, absrep_id = term_absrep_id,
+                         repabs_pseudo_id = term_repabs_pseudo_id,
                          cons_info = tm_cons_info, newty = term_ty,
                          genind_term_REP = genind_term_REP}
 
@@ -88,8 +90,8 @@ val forms_exist = prove(
   qexists_tac `GLAM ARB (ftmRN s) [] []` >>
   match_mp_tac glam >> simp[] >> qexists_tac `[]` >> simp[]);
 
-val {absrep_id, newty = form_ty,
-     repabs_pseudo_id, termP = formP, termP_exists,
+val {absrep_id = form_absrep_id, newty = form_ty,
+     repabs_pseudo_id = form_repabs_pseudo_id, termP = formP, termP_exists,
      termP_term_REP = formP_form_REP,
      term_ABS_t = form_ABS_t, term_ABS_pseudo11 = form_ABS_pseudo11,
      term_REP_t = form_REP_t, term_REP_11} =
@@ -156,8 +158,8 @@ val {tpm_thm = fpm_thm0, term_REP_tpm = form_REP_fpm, t_pmact_t = f_pmact_t,
      tpm_t = fpm_t} =
     define_permutation { name_pfx = "f", name = "form",
                          term_REP_t = form_REP_t,
-                         term_ABS_t = form_ABS_t, absrep_id = absrep_id,
-                         repabs_pseudo_id = repabs_pseudo_id,
+                         term_ABS_t = form_ABS_t, absrep_id = form_absrep_id,
+                         repabs_pseudo_id = form_repabs_pseudo_id,
                          cons_info = fm_cons_info, newty = form_ty,
                          genind_term_REP = formP_form_REP}
 
@@ -169,6 +171,119 @@ val fpm_thm = save_thm(
                             GSYM listTheory.MAP_MAP_o]
            |> REWRITE_RULE [REL_def'])
 
+(* support *)
+val term_REP_eqv = prove(
+   ``support (fn_pmact ^t_pmact_t gt_pmact) ^term_REP_t {}`` ,
+   srw_tac [][support_def, fnpm_def, FUN_EQ_THM, term_REP_tpm, pmact_sing_inv]);
+
+val supp_term_REP = prove(
+  ``supp (fn_pmact ^t_pmact_t gt_pmact) ^term_REP_t = {}``,
+  REWRITE_TAC [GSYM pred_setTheory.SUBSET_EMPTY] >>
+  MATCH_MP_TAC (GEN_ALL supp_smallest) >>
+  srw_tac [][term_REP_eqv])
+
+val tpm_def' =
+    term_REP_tpm |> AP_TERM term_ABS_t |> PURE_REWRITE_RULE [term_absrep_id]
+
+val t = mk_var("t", term_ty)
+val supptpm_support = prove(
+  ``support ^t_pmact_t ^t (supp gt_pmact (^term_REP_t ^t))``,
+  srw_tac [][support_def, tpm_def', supp_fresh, term_absrep_id]);
+
+val supptpm_apart = prove(
+  ``x ∈ supp gt_pmact (^term_REP_t ^t) ∧ y ∉ supp gt_pmact (^term_REP_t ^t) ⇒
+    ^tpm_t [(x,y)] ^t ≠ ^t``,
+  srw_tac [][tpm_def']>>
+  DISCH_THEN (MP_TAC o AP_TERM term_REP_t) >>
+  srw_tac [][term_repabs_pseudo_id, genind_gtpm_eqn, genind_term_REP,
+             supp_apart]);
+
+val supp_tpm = prove(
+  ``supp ^t_pmact_t ^t = supp gt_pmact (^term_REP_t ^t)``,
+  match_mp_tac (GEN_ALL supp_unique_apart) >>
+  srw_tac [][supptpm_support, supptpm_apart, FINITE_GFV])
+
+val supp_tpml = prove(
+  ``supp (list_pmact ^t_pmact_t) ts = GFVl (MAP foterm_REP ts)``,
+  Induct_on `ts` >> simp[supp_tpm]);
+
+val _ = overload_on ("tFV", ``supp ^t_pmact_t``)
+val _ = overload_on ("tFVl", ``supp (list_pmact ^t_pmact_t)``)
+
+val FINITE_tFV = store_thm(
+  "FINITE_tFV",
+  ``FINITE (tFV t)``,
+  srw_tac [][supp_tpm, FINITE_GFV]);
+val _ = export_rewrites ["FINITE_tFV"]
+
+fun supp_clause repabs_pseudo_id {con_termP, con_def} = let
+  open pred_setTheory
+  val t = mk_comb(``supp ^t_pmact_t``, lhand (concl (SPEC_ALL con_def)))
+in
+  t |> REWRITE_CONV [supp_tpm, con_def, MATCH_MP repabs_pseudo_id con_termP,
+                     GFV_thm]
+    |> REWRITE_RULE [supp_listpm, EMPTY_DELETE, UNION_EMPTY]
+    |> REWRITE_RULE [GSYM supp_tpm, GSYM supp_tpml]
+    |> GEN_ALL
+end
+
+val tFV_thm = Save_thm(
+  "tFV_thm",
+  LIST_CONJ (map (supp_clause term_repabs_pseudo_id) tm_cons_info))
+
+val form_REP_eqv = prove(
+   ``support (fn_pmact ^f_pmact_t gt_pmact) ^form_REP_t {}`` ,
+   srw_tac [][support_def, fnpm_def, FUN_EQ_THM, form_REP_fpm, pmact_sing_inv]);
+
+val supp_form_REP = prove(
+  ``supp (fn_pmact ^f_pmact_t gt_pmact) ^form_REP_t = {}``,
+  REWRITE_TAC [GSYM pred_setTheory.SUBSET_EMPTY] >>
+  MATCH_MP_TAC (GEN_ALL supp_smallest) >>
+  srw_tac [][form_REP_eqv])
+
+val fpm_def' =
+    form_REP_fpm |> AP_TERM form_ABS_t |> PURE_REWRITE_RULE [form_absrep_id]
+
+val t = mk_var("f", form_ty)
+val supptpm_support = prove(
+  ``support ^f_pmact_t ^t (supp gt_pmact (^form_REP_t ^t))``,
+  srw_tac [][support_def, fpm_def', supp_fresh, form_absrep_id]);
+
+val supptpm_apart = prove(
+  ``x ∈ supp gt_pmact (^form_REP_t ^t) ∧ y ∉ supp gt_pmact (^form_REP_t ^t) ⇒
+    ^fpm_t [(x,y)] ^t ≠ ^t``,
+  srw_tac [][fpm_def']>>
+  DISCH_THEN (MP_TAC o AP_TERM form_REP_t) >>
+  srw_tac [][form_repabs_pseudo_id, genind_gtpm_eqn, formP_form_REP,
+             supp_apart]);
+
+val supp_tpm = prove(
+  ``supp ^f_pmact_t ^t = supp gt_pmact (^form_REP_t ^t)``,
+  match_mp_tac (GEN_ALL supp_unique_apart) >>
+  srw_tac [][supptpm_support, supptpm_apart, FINITE_GFV])
+
+val _ = overload_on ("fFV", ``supp ^f_pmact_t``)
+
+val FINITE_fFV = store_thm(
+  "FINITE_fFV",
+  ``FINITE (fFV f)``,
+  srw_tac [][supp_tpm, FINITE_GFV]);
+val _ = export_rewrites ["FINITE_fFV"]
+
+fun supp_clause repabs_pseudo_id {con_termP, con_def} = let
+  open pred_setTheory
+  val t = mk_comb(``supp ^f_pmact_t``, lhand (concl (SPEC_ALL con_def)))
+in
+  t |> REWRITE_CONV [supp_tpm, con_def, MATCH_MP repabs_pseudo_id con_termP,
+                     GFV_thm]
+    |> REWRITE_RULE [supp_listpm, EMPTY_DELETE, UNION_EMPTY]
+    |> REWRITE_RULE [GSYM supp_tpm, GSYM supp_tpml]
+    |> GEN_ALL
+end
+
+val fFV_thm = Save_thm(
+  "fFV_thm",
+  LIST_CONJ (map (supp_clause form_repabs_pseudo_id) fm_cons_info))
 
 
 val _ = export_theory()
